Version avec du typage extrinsèque, on va tenter une version avec typage intrinsèque.

src/Prelude/ListCRM.v
@@ -1,54 +1,58 @@
 Require Import List.
 Import ListNotations.
+From Stdlib Require Import Program.Equality.
 
-Inductive forall_l {A : Type} (P : A -> Prop) : list A -> Prop :=
+Inductive forall_l {A : Type} (P : A -> Type) : list A -> Type :=
 | forall_nil : forall_l P []
 | forall_cons : forall {a : A} {l : list A},
     P a -> forall_l P l -> forall_l P (a :: l).
 
+Inductive In_s {A : Type} : A -> list A -> Type :=
+| In_hd : forall {a : A} {l : list A}, In_s a (a :: l)
+| In_cs : forall {a b : A} {l : list A},
+    In_s a l -> In_s a (b :: l).
+
 Lemma map_forall {A B : Type} :
-  forall (P : A -> Prop) (Q : B -> Prop) (f : A -> B),
+  forall (P : A -> Type) (Q : B -> Type) (f : A -> B),
     (forall a : A, P a -> Q (f a)) ->
     forall l : list A, forall_l P l -> forall_l Q (map f l).
 Proof.
   intros. induction l.
   - constructor.
-  - simpl. inversion H0; subst. constructor.
-    apply H. apply H3.
-    apply IHl. apply H4.
-Qed.
+  - simpl. inversion X0; subst. constructor.
+    apply X. apply X1.
+    apply IHl. apply X2.
+Defined.
 
 Lemma map_forall_rev {A B : Type} :
-  forall (P : A -> Prop) (Q : B -> Prop) (f : A -> B),
+  forall (P : A -> Type) (Q : B -> Type) (f : A -> B),
     (forall a : A, Q (f a) -> P a) ->
     forall l : list A, forall_l Q (map f l) -> forall_l P l.
 Proof.
   intros. induction l. constructor.
-  inversion H0. subst. constructor.
-  apply H. apply H3. apply IHl. apply H4.
-Qed.
+  inversion X0. subst. constructor.
+  apply X. apply X1. apply IHl. apply X2.
+Defined.
 
 Lemma In_forall {A : Type} :
-  forall (P : A -> Prop) (l : list A) (a : A),
-    forall_l P l -> In a l -> P a.
+  forall (P : A -> Type) (l : list A) (a : A),
+    forall_l P l -> In_s a l -> P a.
 Proof.
-  intros. induction l. inversion H0.
-  simpl in H0. destruct H0. subst.
-  inversion H; subst. apply H2.
-  apply IHl. inversion H; subst. apply H4.
-  apply H0.
-Qed.
+  intros. induction X0.
+  inversion X. apply X0.
+  apply IHX0. inversion X. apply X2.
+Defined.
 
 Lemma forall_head {A : Type} :
-  forall (P : A -> Prop) (l : list A) (a : A),
+  forall (P : A -> Type) (l : list A) (a : A),
     forall_l P (a :: l) -> P a.
 Proof.
-  intros. inversion H. apply H2.
-Qed.
+  intros. inversion X. apply X0.
+Defined.
 
 Lemma forall_tail {A : Type} :
-  forall (P : A -> Prop) (l : list A) (a : A),
+  forall (P : A -> Type) (l : list A) (a : A),
     forall_l P (a :: l) -> forall_l P l.
 Proof.
-  intros. inversion H. apply H3.
-Qed.
+  intros. inversion X. apply X1.
+Defined.
